spark2cmproofs.v
@@ -3573,17 +3573,30 @@ Proof.
       * (* Case where No error occured during the whole function call *)
 
         set (sp_proc := Values.Vptr sp0 Int.zero) in *.
-        (* The predicate characterizing the addresses that are not accessible
-           from the called function everything that was free in m at first, and  *)
 
-        XXX FIX THIS DEFINITION.
-        set (forbidden := λ CE sp m sp_id ofs_id,
-                          invisible_cminor_addr st CE g astnum e sp m sp_id ofs_id
-                          /\ ~ is_free_block m sp_id ofs_id).
+        (* Addresses that should be untouched by a function call:
+           the one invisible from the function called except the
+           ones that were free at calling time. This exception is
+           mainly to allow the modification of the chaining variable
+           in the local stack. This chainging variable is invisible
+           (it does not correspond to a spark variable) but it can be
+           changed. In the future this may also include things allocated
+           during the function called (optimization of out argument of
+           type array for instance?).
+           Moreover at the end of the function call, the frame used for it
+           was indeed free at call time, so forbidden mcaller mcallee is
+           strictly included in forbidden m m.
+*)
+        Definition forbidden := λ st CE g astnum e sp m_caller m_callee sp_id ofs_id,
+                                invisible_cminor_addr st CE g astnum e sp m_callee sp_id ofs_id
+                                ∧ ~is_free_block m_caller sp_id ofs_id.
+        Definition forbidden_strict := λ st CE g astnum e sp m_callee sp_id ofs_id,
+                                invisible_cminor_addr st CE g astnum e sp m_callee sp_id ofs_id.
+
 
         up_type.
 
-        assert (h_unchanged_pre_chain:Mem.unchanged_on (forbidden CE sp m) m m_pre_chain).
+        assert (h_unchanged_pre_chain:Mem.unchanged_on (forbidden st CE g astnum e sp m m_chain) m m_pre_chain).
         { (* Lemma about invisible and alloc. *)
           eapply Mem.alloc_unchanged_on.
           eauto. }
@@ -3591,7 +3604,7 @@ Proof.
         (* Since the chaining param is not the translation of a spark variable, 
            we stay in callers environment, that is: from m1 to m4 there is no change
            in the addresses visible in m. *)
-        assert (Mem.unchanged_on (forbidden CE sp m) m_pre_chain m_chain).
+        assert (Mem.unchanged_on (forbidden st CE g astnum e sp m m_chain) m_pre_chain m_chain).
         { unfold chain_param in h_exec_stmt_chain_param.
           !inversion h_exec_stmt_chain_param.
           unfold Mem.storev in heq_storev_v_m_chain.
@@ -3608,9 +3621,147 @@ Proof.
           red.
           intro.
           eapply fresh_block_alloc_perm;eauto. }
-        
-        admit.
-        (*assert (Mem.unchanged_on
+
+        assert (Mem.unchanged_on (forbidden st CE g astnum e sp m m_chain) m_chain m_bdy).
+        { assert (Mem.unchanged_on (forbidden st CE g astnum e sp m_chain m_chain) m_chain m_bdy).
+          { !inversion h_exec_stmt_init;subst.
+            rename m1 into m_initparams.
+            assert (Mem.unchanged_on (forbidden st CE g astnum e sp m_chain m_chain) m_chain m_initparams).
+            {
+
+Axiom trans_unchanged : forall P, transitive _ (Mem.unchanged_on P).
+
+Instance unchanged_on_iff: Proper ((eq ==> eq ==> iff) ==> (eq ==> eq ==> iff)) Mem.unchanged_on.
+Proof.
+  repeat red.
+  !intros P Q;!intros ;subst.
+  split;intros h;auto.
+  - repeat red in H.
+    inversion h.
+    constructor;intros .
+    + eapply unchanged_on_perm;auto.
+      specialize (H b b eq_refl ofs ofs eq_refl).
+      destruct H.
+      eauto.
+    + eapply unchanged_on_contents;auto.
+      specialize (H b b eq_refl ofs ofs eq_refl).
+      destruct H.
+      eauto.
+  - repeat red in H.
+    inversion h.
+    constructor;intros .
+    + eapply unchanged_on_perm;auto.
+      specialize (H b b eq_refl ofs ofs eq_refl).
+      destruct H.
+      eauto.
+    + eapply unchanged_on_contents;auto.
+      specialize (H b b eq_refl ofs ofs eq_refl).
+      destruct H.
+      eauto.
+Qed.
+
+Definition unchange_forbidden st CE g astnum e_chain e_chain' sp m_chain m'_chain :=
+  forall (sp_id : Values.block) (ofs_id : Z),
+    (forbidden st CE g astnum e_chain sp m_chain  m_chain   sp_id ofs_id <->
+     forbidden st CE g astnum e_chain' sp m'_chain m'_chain sp_id ofs_id).
+
+
+Definition strict_unchanged_on st CE g astnum e_chain e_chain' sp m m' :=
+  Mem.unchanged_on (forbidden st CE g astnum e_chain sp m m) m m' /\
+  unchange_forbidden st CE g astnum e_chain e_chain' sp m m'.
+
+
+Lemma exec_store_params_preserve_forbidden:
+  forall lparams st CE initparams,
+    store_params st CE lparams = OK initparams -> 
+    forall astnum g proc_t sp e_chain e_chain' m t2 m' Out_normal,
+      exec_stmt g proc_t sp e_chain m initparams t2 e_chain' m' Out_normal ->
+      unchange_forbidden st CE g astnum e_chain e_chain' sp m m'.
+Proof.
+Admitted.
+
+Lemma exec_store_params_unchanged_on:
+  forall lparams st CE initparams,
+    store_params st CE lparams = OK initparams -> 
+    forall astnum g proc_t sp e_chain m t2 e_postchain m' Out_normal,
+      exec_stmt g proc_t sp e_chain m initparams t2 e_postchain m' Out_normal ->
+      Mem.unchanged_on (forbidden st CE g astnum e_chain sp m m) m m'.
+Proof.
+  !!intros ? ? ?.
+  rewrite store_params_ok.
+  !functional induction (function_utils.store_params st CE lparams);
+    try discriminate;try rewrite <- function_utils.store_params_ok in *; !intros.
+  - !inversion heq;subst.
+    !inversion h_exec_stmt_initparams_Out_normal.
+    apply Mem.unchanged_on_refl.
+  - specialize (IHr x0 heq).
+    !invclear heq1.
+    !inversion h_exec_stmt_initparams_Out_normal;subst;clear h_exec_stmt_initparams_Out_normal.
+    + rename m1 into m_chain'.
+      rename e1 into e_chain'.
+      rename x0 into lparams'_t.
+      up_type.
+      apply trans_unchanged with m_chain'.
+      * !inversion h_exec_stmt;subst.
+        unfold Mem.storev in heq_storev_v_m_chain'.
+        destruct x1_v;try discriminate.
+        apply Mem.store_unchanged_on with (1:=heq_storev_v_m_chain').
+        !intros.
+        (*         unfold sp_proc in h_CM_eval_expr_vaddr. *)
+        !destruct h_and.
+        up_type.
+        intro abs.
+        destruct abs as (abs1, abs2). 
+        red in abs1.
+        !functional inversion heq_transl_name;subst.
+        rewrite <- (transl_variable_astnum _ _ 0%nat _ _ heq_transl_variable astnum) in heq_transl_variable.
+        specialize (abs1 _ _ _ _ _ heq_transl_variable heq_compute_chnk h_CM_eval_expr_x1_x1_v).
+        decomp abs1;try omega;now auto.          
+      * enough (Mem.unchanged_on (forbidden st CE g astnum e_chain' sp m_chain' m_chain') m_chain' m').
+        { !!pose proof exec_store_params_preserve_forbidden.
+          specialize (H0 _ _ _ _ heq astnum _ _ _ _ _ _ _ _ _ h_exec_stmt_x0_Out_normal).
+          red in H0.
+          symmetry in H0.
+          eapply unchanged_on_iff;eauto.
+          do 2 red;intros;subst.
+          split;intros .
+          eapply H0;eauto.
+          - 
+          red.
+        !intros.
+        unfold forbidden.
+        }
+        eapply IHr;eauto.
+      * eapply IHr.
+    + (*an error occurred during the first param.*)
+Qed.
+
+λ CE sp m_caller m_callee sp_id ofs_id, invisible_cminor_addr st CE g astnum e sp m_callee sp_id ofs_id
+
+ rewrite store_params_ok in heq_store_prms_lparams_x3.
+              !functional induction (function_utils.store_params st CE_proc lparams);
+                try discriminate.
+              - !inversion heq_store_prms_lparams_x3;subst.
+                !inversion h_exec_stmt_initparams.
+                apply Mem.unchanged_on_refl.
+              - 
+                fold tlparams in IHr.
+                fold proc_t in IHr.
+                  set (porc_t' :=
+                         {|
+                           fn_sig := x5;
+                           fn_params := chaining_param 
+                                          :: transl_lparameter_specification_to_lident st lparams';
+                           fn_vars := transl_decl_to_lident st decl;
+                           fn_stackspace := proc_sz_locals;
+                           fn_body := pbody_t |})
+                  in *.
+            }
+
+          }
+        }
+
+        assert (Mem.unchanged_on
                   (λ sp_id ofs_id,
                    invisible_cminor_addr st CE_proc g astnum e sp m sp_id ofs_id)
                   m m1).
@@ -3619,7 +3770,7 @@ Proof.
         admit. (* associativity of unchanged_on? No, more
                                 complex: the unchanged_on on the body part
                                 correpsond to either visible parts from sp or from
-                                freeed space (outcome_free_mem m2 ... m'). *) *)
+                                freeed space (outcome_free_mem m2 ... m'). *)
 
       * eq_same_clear.
       * (* init phase raised an error. *)
