spark2Cminor.v
@@ -890,8 +890,8 @@ Fixpoint transl_procedure (stbl:symboltable) (enclosingCE:compilenv)
           (* we formulate the sequence as Sseq (initializing, Sseq (bdy copyout)) to ease proofs. *)
           let proc_t :=
               Sseq chain_param
-                   (Sseq (Sseq initparams (Sseq locvarinit bdy))
-                         copyout) in
+                   (Sseq (Sseq initparams (Sseq locvarinit Sskip))
+                         (Sseq bdy copyout)) in
                 
           do procsig <- transl_lparameter_specification_to_procsig stbl lvl lparams ;
           (** For a given "out" (or inout) argument x of type T of a procedure P:
